@@ -20,8 +20,7 @@ def memcpyAddr : BitVec 64 := BitVec.ofNat 64 KernelSyms.«memcpy»
 
 /-- **WP of `memcpy`.** -/
 def wp_memcpy_body {hlc : HasLC} {GF : BundledGFunctors} [MachGS hlc GF] [CurCtx]
-    (cpu : CPU) (k : KCtx) (bs olds : List (BitVec 8)) (n : Nat) (dqs : DFrac)
-    (hsie : k.sie = false) (hK : 4 ≤ k.avail)
+    (cpu : CPU) (k : KCtx) (bs olds : List (BitVec 8)) (n : Nat) (dqs : DFrac) (hK : 4 ≤ k.avail)
     (hn : k.regs 12#5 = BitVec.ofNat 64 n) (hn32 : n < 2 ^ 32)
     (hls : bs.length = n) (hld : olds.length = n) : Prop :=
   kctx cpu k ∗ pcIs cpu memcpyAddr ∗
@@ -36,7 +35,7 @@ def wp_memcpy_body {hlc : HasLC} {GF : BundledGFunctors} [MachGS hlc GF] [CurCtx
 structure MEMCPY : Prop where
   wp_memcpy : ∀ {hlc : HasLC} {GF : BundledGFunctors} [MachGS hlc GF] [CurCtx]
     (cpu : CPU) (k : KCtx) (bs olds : List (BitVec 8)) (n : Nat) (dqs : DFrac)
-    hsie hK hn hn32 hls hld,
-    wp_memcpy_body (hlc := hlc) (GF := GF) cpu k bs olds n dqs hsie hK hn hn32 hls hld
+    hK hn hn32 hls hld,
+    wp_memcpy_body (hlc := hlc) (GF := GF) cpu k bs olds n dqs hK hn hn32 hls hld
 
 end Xv6
